The Elimination of Platform.Bytes, Part I.

doc/tutorial/code/exercises/Ex12.SHA1.fst
@@ -16,23 +16,23 @@
 module Ex12.SHA1
 open FStar.All
 open FStar.Seq
-open Platform.Bytes
+open FStar.Bytes
 open CoreCrypto
 
-type text  = bytes    (* a type abbreviation, for clarity *)
+type text  = b:bytes{UInt.fits (length b) 31}    (* a type abbreviation, for clarity *)
 
 
 (* we rely on some external crypto library implementing HMAC-SHA1 *)
 
-let keysize = 16
+let keysize = 16ul
 let blocksize = keysize
-let macsize = 20
+let macsize = 20ul
 
-type key = lbytes keysize
-type tag = bytes //lbytes macsize
+type key = lbytes32 keysize
+type tag = lbytes32 macsize
 
-val sample: n:nat -> ML (lbytes n)
-let sample n = random n 
+val sample: n:UInt32.t -> ML (lbytes32 n)
+let sample n = random32 n 
 
 val sha1 : bytes -> Tot (h:bytes{length h = 20})
 let sha1 b = hash SHA1 b
@@ -41,8 +41,8 @@ val hmac_sha1: key -> text -> Tot tag
 let hmac_sha1 k t =
   let x5c = byte_of_int 92 in
   let x36 = byte_of_int 54 in
-  let opad = createBytes blocksize x5c in
-  let ipad = createBytes blocksize x36 in
+  let opad = create blocksize x5c in
+  let ipad = create blocksize x36 in
   let xor_key_opad = xor keysize k opad in
   let xor_key_ipad = xor keysize k ipad in
   sha1 ( xor_key_opad @|
