doc/tutorial/code/exercises/Ex12a1.Cap.fst
@@ -19,21 +19,23 @@ module Ex12a1.Cap (* capabilities *)
 
 open FStar.ST
 open FStar.All
-open Platform.Bytes
+open FStar.Bytes
 
 
 module ACLs = Ex12a.ACLs
 module MAC = Ex12.MAC
 
 // BEGIN: UTF8Inj
-assume val utf8: s:string  -> Tot bytes
+assume val utf8_encode: s:string  -> Tot bytes
 
 assume UTF8_inj:
-  forall s0 s1.{:pattern (utf8 s0); (utf8 s1)}
-     b2t (equalBytes (utf8 s0) (utf8 s1)) ==> s0==s1
+  forall s0 s1.{:pattern (utf8_encode s0); (utf8_encode s1)}
+     b2t (utf8_encode s0 = utf8_encode s1) ==> s0==s1
 // END: UTF8Inj
 
-type capRead (msg:bytes) = (forall f. msg = utf8 f ==> ACLs.canRead f)
+type string30 = (s:string{ String.length s < pow2 30 })
+
+type capRead (msg:bytes) = (forall (f:string30). msg = utf8_encode f ==> ACLs.canRead f)
 
 let k = MAC.keygen capRead
 
