doc/tutorial/code/exercises/Ex12c.Format.fst
@@ -16,7 +16,7 @@
 module Ex12c.Format
 
 open FStar.String
-open Platform.Bytes         //This shadows length, index etc. from FStar.Seq, for no good reason?
+open FStar.Bytes            //This shadows length, index etc. from FStar.Seq, for no good reason?
 open FStar.Seq              //It's really important for FStar.Seq.index to have precedence for proper use of the lemmas in FStar.Seq
 open FStar.Classical
 
@@ -25,19 +25,19 @@ type msg (l:nat) = lbytes l
 
 (* ----- a lemma on array append *)
 // BEGIN: FormatAppendEx
-val append_inj_lemma: b1:message -> b2:message
-                   -> c1:message -> c2:message
-                   -> Lemma (requires (length b1==length c1 
-		                      /\ b2t (Seq.eq (b1 @| b2) (c1 @| c2))))
-                           (ensures (b2t (Seq.eq b1 c1) /\ b2t (Seq.eq b2 c2)))
-                           [SMTPat (b1 @| b2); SMTPat (c1 @| c2)] 
+val append_inj_lemma: b1:message -> b2:message {UInt.fits (Bytes.length b1 + Bytes.length b2) 32}
+                   -> c1:message -> c2:message {UInt.fits (Bytes.length c1 + Bytes.length c2) 32}
+                   -> Lemma (requires (Bytes.length b1==Bytes.length c1 
+		                      /\ (Bytes.append b1 b2) = (Bytes.append c1 c2)))
+                           (ensures (Bytes.equal b1 c1 /\ Bytes.equal b2 c2))
+                           [SMTPat (Bytes.append b1 b2); SMTPat (Bytes.append c1 c2)] 
 			   (* given to the SMT solver *)
 let append_inj_lemma b1 b2 c1 c2 =
-  lemma_append_len_disj b1 b2 c1 c2;
+  lemma_append_len_disj (reveal b1) (reveal b2) (reveal c1) (reveal c2);
   Classical.forall_intro 
     #_ 
-    #(fun (x:(i:nat{i < length b1})) -> index b1 x == index c1 x) 
-    (lemma_append_inj_l b1 b2 c1 c2); 
+    #(fun (x:(i:nat{i < Bytes.length b1})) -> Bytes.index b1 x == Bytes.index c1 x) 
+    (lemma_append_inj_l (reveal b1) (reveal b2) (reveal c1) (reveal c2)); 
     //currently the 2nd implicit argument has to be provided explicitly
   admit()
 // END: FormatAppendEx
