doc/tutorial/code/solutions/Ex12a2.Cap.fst
@@ -16,36 +16,40 @@
 (* to be used with Ex12.MAC.fst and Ex12a.ACLs.fst *)
 
 module Ex12a2.Cap (* capabilities *) 
+
 open FStar.ST
 open FStar.All
-open Platform.Bytes
-
+open FStar.Bytes
 
 
 module ACLs = Ex12a.ACLs
 module MAC = Ex12.MAC
 
-// In Platform.Bytes: val utf8: s:string  -> Tot bytes
+// In FStar.Bytes: val utf8_encode: s:string  -> Tot bytes
 
 assume UTF8_inj:
-  forall s0 s1.{:pattern (utf8 s0); (utf8 s1)}
-     b2t (equalBytes (utf8 s0) (utf8 s1)) ==> s0==s1
+  forall s0 s1.{:pattern (utf8_encode s0); (utf8_encode s1)}
+     Bytes.equal (utf8_encode s0) (utf8_encode s1) ==> s0==s1
 
-type capRead (msg:bytes) = (forall f. msg = utf8 f ==> ACLs.canRead f)
+type string30 = (s:string{ String.length s < pow2 30 })
+
+type capRead (msg:bytes) = (forall (f:string30). msg = utf8_encode f ==> ACLs.canRead f)
 
 let k_read = MAC.keygen capRead
 
-val issue_read: f:string{ ACLs.canRead f } -> ML MAC.tag
-val redeem_read: f:string -> m:MAC.tag -> ML (u:unit{ ACLs.canRead f })
+val issue_read: f:string30{ ACLs.canRead f } -> ML MAC.tag
+val redeem_read: f:string30 -> m:MAC.tag -> ML (u:unit{ ACLs.canRead f })
 
 let issue_read f =
   assert(ACLs.canRead f);
-  let bs = (utf8 f) in
+  let bs = (utf8_encode f) in
   assert(capRead bs);
+  assume (Bytes.length bs < pow2 30);
   MAC.mac k_read bs
 
 let redeem_read f t =
-  let bs = (utf8 f) in
+  let bs = (utf8_encode f) in
+  assume (Bytes.length bs < pow2 30);
   if MAC.verify k_read bs t then
     (MAC.from_key_prop k_read bs ;
     assert (ACLs.canRead f))
@@ -53,22 +57,23 @@ let redeem_read f t =
     failwith "bad capability"
 
 // Begin: CapImplementation2
-type capWrite (msg:bytes) = (forall f. msg = utf8 f ==> ACLs.canWrite f)
+type capWrite (msg:bytes) = (forall (f:string30). msg = utf8_encode f ==> ACLs.canWrite f)
 
 let k_write = MAC.keygen capWrite
 
-val issue_write: f:string{ ACLs.canWrite f } -> ML MAC.tag
-val redeem_write: f:string -> m:MAC.tag -> ML(u:unit{ ACLs.canWrite f })
+val issue_write: f:string30{ ACLs.canWrite f } -> ML MAC.tag
+val redeem_write: f:string30 -> m:MAC.tag -> ML(u:unit{ ACLs.canWrite f })
 
 let issue_write f =
   assert(ACLs.canWrite f);
-  let bs = (utf8 f) in
+  let bs = (utf8_encode f) in
   assert(capWrite bs);
+  assume (Bytes.length bs < pow2 30);
   MAC.mac k_write bs
 
-
 let redeem_write f t =
-  let bs = (utf8 f) in
+  let bs = (utf8_encode f) in
+  assume (Bytes.length bs < pow2 30);
   if MAC.verify k_write bs t then
     (MAC.from_key_prop k_write bs ;
     assert(ACLs.canWrite f))
