doc/tutorial/code/solutions/Ex12b2.Format.fst
@@ -16,27 +16,23 @@
 module Ex12b2.Format
 
 open FStar.String
-open Platform.Bytes         //This shadows length, index etc. from FStar.Seq, for no good reason?
+open FStar.Bytes            //This shadows length, index etc. from FStar.Seq, for no good reason?
 open FStar.Seq              //It's really important for FStar.Seq.index to have precedence for proper use of the lemmas in FStar.Seq
 open FStar.Classical
 
-// BEGIN: FormatMsg
 type message = bytes
 type msg (l:nat) = lbytes l
-// END: FormatMsg
 
 (* ----- a lemma on array append *)
-// BEGIN: FormatAppend
-val append_inj_lemma: b1:message -> b2:message
-                   -> c1:message -> c2:message
-                   -> Lemma (requires (length b1==length c1 /\ b2t (Seq.eq (b1 @| b2) (c1 @| c2))))
-                            (ensures (b2t (Seq.eq b1 c1) /\ b2t (Seq.eq b2 c2)))
-                            [SMTPat (b1 @| b2); SMTPat (c1 @| c2)] (* given to the SMT solver *)
-// END: FormatAppend
+val append_inj_lemma: b1:message -> b2:message {UInt.fits (Bytes.length b1 + Bytes.length b2) 32}
+                   -> c1:message -> c2:message {UInt.fits (Bytes.length c1 + Bytes.length c2) 32}
+                   -> Lemma (requires (Bytes.length b1==Bytes.length c1 /\ b2t ((Bytes.append b1 b2) = (Bytes.append c1 c2))))
+                            (ensures (Bytes.equal b1 c1 /\ Bytes.equal b2 c2))
+                            [SMTPat (Bytes.append b1 b2); SMTPat (Bytes.append c1 c2)] (* given to the SMT solver *)
 let append_inj_lemma b1 b2 c1 c2 =
-  lemma_append_len_disj b1 b2 c1 c2;
-  Classical.forall_intro #_ #(fun (x:(i:nat{i < length b1})) -> index b1 x == index c1 x) (lemma_append_inj_l b1 b2 c1 c2); //sadly, the 2nd implicit argument has to be provided explicitly
-  Classical.forall_intro #_ #(fun (x:(i:nat{i < length b2})) -> index b2 x == index c2 x) (lemma_append_inj_r b1 b2 c1 c2)  //should fix this soon (NS)
+  lemma_append_len_disj (reveal b1) (reveal b2) (reveal c1) (reveal c2);
+  Classical.forall_intro #_ #(fun (x:(i:nat{i < Bytes.length b1})) -> Bytes.index b1 x == Bytes.index c1 x) (lemma_append_inj_l (reveal b1) (reveal b2) (reveal c1) (reveal c2)); //sadly, the 2nd implicit argument has to be provided explicitly
+  Classical.forall_intro #_ #(fun (x:(i:nat{i < Bytes.length b2})) -> Bytes.index b2 x == Bytes.index c2 x) (lemma_append_inj_r (reveal b1) (reveal b2) (reveal c1) (reveal c2))  //should fix this soon (NS)
 
 abstract val lemma_eq_intro: #a:Type -> s1:seq a -> s2:seq a -> Lemma
      (requires (Seq.length s1 = Seq.length s2
@@ -56,39 +52,43 @@ type uint16 = i:int{uInt16 i}
 let utf8 s = magic()*)
 
 (*val iutf8: m:message -> s:string{utf8 s == m}
-let iutf8 m = Platform.Bytes.iutf8 m*)
+let iutf8 m = FStar.Bytes.iutf8 m*)
 
 assume UTF8_inj:
-  forall s0 s1.{:pattern (utf8 s0); (utf8 s1)}
-    b2t (Seq.eq (utf8 s0) (utf8 s1)) ==> s0==s1
+  forall s0 s1.{:pattern (utf8_encode s0); (utf8_encode s1)}
+    Bytes.equal (utf8_encode s0) (utf8_encode s1) ==> s0==s1
 
 val uint16_to_bytes: u:uint16{repr_bytes u <= 2} -> Tot (msg 2)
 
 let uint16_to_bytes u = bytes_of_int 2 u
 
-assume UINT16_inj: forall s0 s1. b2t (Seq.eq (uint16_to_bytes s0) (uint16_to_bytes s1)) ==> s0==s1
+assume UINT16_inj: forall s0 s1. Bytes.equal (uint16_to_bytes s0) (uint16_to_bytes s1) ==> s0==s1
 
-type string16 = s:string{uInt16 (length (utf8 s))} (* up to 65K *)
-
+type string16 = s:string{uInt16 (String.length s)} (* up to 65K *)
+type string30 = (s:string{UInt.fits (String.length s) 30}) 
 
 (* =============== the formatting we use for authenticated RPCs *)
 
-// BEGIN: FormatReqRes
-val request : string -> Tot message
-val response: string16 -> string -> Tot message
+val request : string30 -> Tot message
+val response: (s:string16{UInt.fits (String.length s) 16}) -> string30 -> Tot message
 
 (* -------- implementation *)
 
-let tag0 = createBytes 1 0uy
-let tag1 = createBytes 1 1uy
+let tag0 = Bytes.create 1ul 0uy
+let tag1 = Bytes.create 1ul 1uy
 
-let request s = tag0 @| (utf8 s)
+let request s = Bytes.append tag0 (utf8_encode s)
 
 let response s t =
-  lemma_repr_bytes_values (length (utf8 s));
-  let lb = uint16_to_bytes (length (utf8 s)) in
-  tag1 @| (lb @| ( (utf8 s) @| (utf8 t)))
-// END: FormatReqRes
+  let us = utf8_encode s in
+  let lus = min (Bytes.length us) 65535 in
+  lemma_repr_bytes_values lus;
+  let lb = uint16_to_bytes lus in
+  let us = utf8_encode s in
+  let ut = utf8_encode t in
+  assume (UInt.fits (Bytes.length us + Bytes.length ut) 30);
+  Bytes.append tag1 (Bytes.append lb (Bytes.append us ut))
+
 
 (* ------- 3 lemmas on message formats:
 
@@ -100,36 +100,30 @@ let response s t =
    functions---they just return messages---so these three lemmas are
    sufficient *)
 
-// BEGIN: FormatLemmas
+
 val req_resp_distinct:
-  s:string -> s':string16 -> t':string ->
+  s:string30 -> s':string16 -> t':string30 ->
   Lemma (requires True)
         (ensures (request s <> response s' t'))
         [SMTPat (request s); SMTPat (response s' t')]
 
 val req_injective:
-  s0:string -> s1:string ->
-  Lemma (requires (b2t (Seq.eq (request s0) (request s1))))
+  s0:string30 -> s1:string30 ->
+  Lemma (requires (Bytes.equal (request s0) (request s1)))
         (ensures  (s0==s1))
         (*[SMTPat (request s0); SMTPat (request s1)]*)
 
 val resp_injective:
-  s0:string16 -> t0:string -> s1:string16 -> t1:string ->
-  Lemma (requires (b2t (Seq.eq (response s0 t0) (response s1 t1))))
+  s0:string16 -> t0:string30 -> s1:string16 -> t1:string30 ->
+  Lemma (requires (Bytes.equal (response s0 t0) (response s1 t1)))
         (ensures  (s0==s1 /\ t0==t1))
         [SMTPat (response s0 t0); SMTPat (response s1 t1)]
-// END: FormatLemmas
 
-// BEGIN: FormatProofs
-let req_resp_distinct s s' t' = 
-  lemma_repr_bytes_values (length (utf8 s));
-  lemma_repr_bytes_values (length (utf8 s'));
-  assert (Seq.index (request s) 0 == 0uy);
-  assert (Seq.index (response s' t') 0 == 1uy)
 
-let req_injective s0 s1 = ()
+// BEGIN: FormatProofsEx
+let req_resp_distinct s s' t' = admit()
 
-let resp_injective s0 t0 s1 t1 =
-  lemma_repr_bytes_values (length (utf8 s0));
-  lemma_repr_bytes_values (length (utf8 s1))
-// END: FormatProofs
+let req_injective s0 s1 = admit()
+
+let resp_injective s0 t0 s1 t1 = admit()
+// END: FormatProofsEx
