ucontrib/CoreCrypto/fst/CoreCrypto.fst
@@ -15,7 +15,7 @@
 *)
 module CoreCrypto
 
-open Platform.Bytes
+open FStar.Bytes
 
 (* ------------ Hashing ------------ *)
 type hash_alg =
